Uniana.v
@@ -31,20 +31,23 @@ Module Uniana.
       uni_state_concr (abs_uni_eff uni) qs qs'.
 
   Definition uni_concr (u : Uni) : Hyper :=
-    fun ts => forall t t' tr tr', ts t tr -> ts t' tr' ->
-                          forall x p i s s', In t tr ((p, i), s) ->
-                                        In t' tr' ((p, i), s') ->
-                                        u p x = true -> s x = s' x.
+    fun ts => forall t t', ts t -> ts t' ->
+                   forall x p i s s', In (p, i, s) (`t) ->
+                                 In (p, i, s') (`t') ->
+                                 u p x = true -> s x = s' x.
   
   Definition uni_trans (uni : Uni) (upi : Upi) (unch : Unch) : Uni :=
-    fun p => if p == root then uni root
-             else fun x => ((join_andb (map (fun spl => 
-                                           match spl with (s, x) => uni s x &&
-                                                upi_trans upi uni s p end) (splits p))) 
-                              && (join_andb (map (fun q => abs_uni_eff (uni q) x) (preds p)))
-                              && (join_andb (map (fun q => upi_trans upi uni q p) (preds p)))
-                           )
-                        || join_orb (map (fun q => (q <>b p) && uni q x && upi_trans upi uni q p) (unch_trans unch p x)).
+    fun p
+    => if p == root then uni root
+      else fun x => ((join_andb (map (fun spl => match spl with
+                                             (s, x) => uni s x && upi_trans upi uni s p
+                                           end)
+                                  (splits p)))
+                    && (join_andb (map (fun q => abs_uni_eff (uni q) x) (preds p)))
+                    && (join_andb (map (fun q => upi_trans upi uni q p) (preds p)))
+                 )
+                 || join_orb (map (fun q => (q <>b p) && uni q x && upi_trans upi uni q p)
+                                 (unch_trans unch p x)).
 
   Lemma uni_trans_root_inv :
     forall uni hom unch x, uni_trans uni hom unch root x = uni root x.
@@ -57,29 +60,29 @@ Module Uniana.
   Qed.
 
   Lemma uni_correct :
-    forall uni upi unch t,
-        sem_hyper (red_prod (red_prod (uni_concr uni) (upi_concr upi)) (lift (unch_concr unch))) t ->
-        uni_concr (uni_trans uni upi unch) t.
+    forall uni upi unch ts,
+        sem_hyper (red_prod (red_prod (uni_concr uni) (upi_concr upi)) (lift (unch_concr unch))) ts ->
+        uni_concr (uni_trans uni upi unch) ts.
   Proof.
-    intros uni upi unch t Hred.
+    intros uni upi unch ts Hred.
     unfold sem_hyper in Hred.
-    destruct Hred as [ts [Hconcr Hstep]].
-    intros k k' tr tr' Hsem Hsem' x p i s s'.
-    intros HIn HIn' Htrans.
+    destruct Hred as [ts' [Hconcr Hstep]].
+    unfold uni_concr.
+    intros t t' Hsem Hsem' x p i s s' HIn HIn' Htrans.
 
-    assert (upi_concr (upi_trans upi uni) t) as HCupi. {
+    assert (upi_concr (upi_trans upi uni) ts) as HCupi. {
       apply upi_correct. 
       destruct Hconcr as [[_ Hhom] _].
-      exists ts; auto.
+      exists ts'; auto.
     }
 
-    assert (unch_concr (unch_trans unch) k tr) as HCunch. {
+    assert (unch_concr (unch_trans unch) t) as HCunch. {
       destruct Hconcr as [[_ _] Hunch].
       unfold lift in *; subst.
       apply unch_correct. assumption.
     } 
     
-    assert (unch_concr (unch_trans unch) k' tr') as HCunch'. {
+    assert (unch_concr (unch_trans unch) t') as HCunch'. {
       destruct Hconcr as [[_ _] Hunch].
       unfold lift in *; subst.
       apply unch_correct. assumption.
@@ -89,38 +92,54 @@ Module Uniana.
 
     subst.
     unfold uni_trans in Htrans. 
-    assert (X := Hsem). destruct X as [l [ltr [lstep [Hts Hlstep]]]]; subst.
-    assert (X := Hsem'). destruct X as [l' [ltr' [lstep' [Hts' Hlstep']]]]; subst.
-
+    assert (X := Hsem). destruct X as [t1 [k1 [Hts1 Hteq1]]].
+    (*destruct X as [l [ltr [lstep [Hts Hlstep]]]]; subst.*)
+    assert (X := Hsem'). destruct X as [t2 [k2 [Hts2 Hteq2]]].
+    (*destruct X as [l' [ltr' [lstep' [Hts' Hlstep']]]]; subst.*)
     destruct (p == root); [ subst | ].
-    + rewrite e in *; clear e.
-      inv_tr HIn.
-      - exfalso. eauto using start_no_tgt. 
-      - inv_tr HIn'; [ exfalso |]; eauto using start_no_tgt. 
-
-    + conv_bool.
+    - rewrite e in *; clear e. 
+      (*destruct t as [t tr]. destruct t; cbn in HIn; inversion HIn.*)
+      eapply HCuni; [eapply Hts1|apply Hts2| | | apply Htrans].
+      + specialize (root_prefix t1) as [s0 rp]. apply root_start_tag in HIn as rst. subst i.
+        eapply prefix_cons_in in rp as rp'.
+        assert (Prefix (`t1) (`t)) as pre_t.
+        { rewrite Hteq1. cbn. econstructor. econstructor. }
+        eapply prefix_trans with (l2:=`t1) (l3:=`t) in rp; eauto.
+        apply prefix_cons_in in rp. eapply tag_inj in HIn; [| apply rp]. subst s0. eauto.
+      + specialize (root_prefix t2) as [s0 rp]. apply root_start_tag in HIn as rst. subst i.
+        eapply prefix_cons_in in rp as rp'.
+        assert (Prefix (`t2) (`t')) as pre_t.
+        { rewrite Hteq2. cbn. econstructor. econstructor. }
+        eapply prefix_trans with (l2:=`t2) (l3:=`t') in rp; eauto.
+        apply prefix_cons_in in rp. eapply tag_inj in HIn'; [| apply rp]. subst s0. eauto.
+    - conv_bool.
       destruct Htrans as [Htrans | Hunch].
-        (* The uni/hom case *)
-      - destruct Htrans as [[Hsplit Hpred] Hupi].
-        eapply in_pred_exists in HIn; try eassumption.
-        eapply in_pred_exists in HIn'; try eassumption.
+      (* The uni/hom case *)
+      + destruct Htrans as [[Hsplit Hpred] Hupi].
+        rewrite Hteq1 in HIn. rewrite Hteq2 in HIn'.
+        eapply in_pred_exists in HIn; try eassumption; [|setoid_rewrite <-Hteq1; exact (proj2_sig t)].
+        eapply in_pred_exists in HIn'; try eassumption;[|setoid_rewrite <-Hteq2; exact (proj2_sig t')].
         destruct HIn as [q [j [r [HIn Hstep]]]].
         destruct HIn' as [q' [j' [r' [HIn' Hstep']]]].
         assert (List.In q (preds p)) as Hqpred by (eauto using step_conf_implies_edge).
-
         cut (q' = q); intros; subst.
         * cut (j' = j); intros; subst.
           -- eapply (local_uni_corr (uni q) q j p i r r' s s'); try eassumption.
              ** unfold uni_state_concr. intros.
                 unfold uni_concr in HCuni .
-                eapply (HCuni l l' ltr ltr' Hts Hts' x0 q j); eassumption.
+                eapply (HCuni _ _ Hts1 Hts2 x0 q j); eassumption.
              ** eapply join_andb_true_iff in Hpred; try eassumption.
           -- (* unique preceding instances *)
-             eapply join_andb_true_iff in Hupi; try eassumption.
-             assert (p =/= q) by (symmetry; eauto using step_conf_implies_edge, no_self_loops).
-             eapply HCupi; [ eapply Hsem | eapply Hsem' | eassumption | | ].
-             all: eauto using precedes_step.
-        * (* disjoint paths! *)
+            eapply join_andb_true_iff in Hupi; try eassumption.
+            assert (p =/= q) by (symmetry; eauto using step_conf_implies_edge, no_self_loops).
+            symmetry.
+            eapply HCupi; [ eapply Hsem | eapply Hsem' | eassumption | | ].
+            1: rewrite Hteq1. 2: rewrite Hteq2.
+            all: cbn; rewrite nlcons_to_list; eapply precedes_step; eauto.
+            all: rewrite <-nlcons_necons.
+            ++ setoid_rewrite <-Hteq1. destruct t; cbn; eauto.
+            ++ setoid_rewrite <-Hteq2. destruct t'; cbn; eauto.
+        * (* disjoint paths! *) admit. (*
           destruct (q == q') as [ Heq | Hneq ]; [ eauto | exfalso ].
           assert (List.In q' (preds p)) as Hqpred' by (eauto using step_conf_implies_edge).
           unfold upi_concr in HCupi.
@@ -138,9 +157,9 @@ Module Uniana.
           ++ intros.
              eapply HCupi; eauto.
              eapply (join_andb_true_iff _ _ Hsplit) in H.
-             conv_bool. destruct H as [_ H]. eassumption.
+             conv_bool. destruct H as [_ H]. eassumption. *)
         (* The unch case *)
-      - rename Hunch into H.
+      + rename Hunch into H.
         eapply join_orb_true_iff in H.
         destruct H as [u H].
         conv_bool.
@@ -151,8 +170,8 @@ Module Uniana.
         destruct HCunch' as [j' [r' [Hprec' Heq']]]; try eassumption.
         rewrite <- Heq. rewrite <- Heq'.
         cut (j' = j); intros.
-        * subst j'. eauto using precedes_step_inv.  
-        * eapply (HCupi _ _ _ _ Hsem Hsem'); eauto. 
+        * subst j'. admit. (*eauto using precedes_step_inv.  *)
+        * symmetry. eapply (HCupi _ _ Hsem Hsem'); eauto. 
   Qed.
 
 
